Foundation/InterpretabilityLogic/Hilbert/Axiom.lean
@@ -207,22 +207,22 @@ def HasW.of_mem {Ax₁ Ax₂ : Axiom α} (h : Ax₁ ⊆ Ax₂) [Ax₁.HasW] : Ax
   mem_W := h mem_W
 
 
-class HasWStar where
+class HasWstar where
   p : α
   q : α
   r : α
   ne_pq : p ≠ q := by simp;
   ne_qr : q ≠ r := by simp;
   ne_rp : r ≠ p := by simp;
-  mem_WStar : InterpretabilityLogic.Axioms.WStar (.atom p) (.atom q) (.atom r) ∈ Ax := by grind;
-attribute [simp] HasWStar.ne_pq HasWStar.ne_qr HasWStar.ne_rp
-export HasWStar (mem_WStar)
+  mem_Wstar : InterpretabilityLogic.Axioms.Wstar (.atom p) (.atom q) (.atom r) ∈ Ax := by grind;
+attribute [simp] HasWstar.ne_pq HasWstar.ne_qr HasWstar.ne_rp
+export HasWstar (mem_Wstar)
 
-def HasWStar.of_mem {Ax₁ Ax₂ : Axiom α} (h : Ax₁ ⊆ Ax₂) [Ax₁.HasWStar] : Ax₂.HasWStar where
-  p := HasWStar.p Ax₁;
-  q := HasWStar.q Ax₁;
-  r := HasWStar.r Ax₁;
-  mem_WStar := h mem_WStar
+def HasWstar.of_mem {Ax₁ Ax₂ : Axiom α} (h : Ax₁ ⊆ Ax₂) [Ax₁.HasWstar] : Ax₂.HasWstar where
+  p := HasWstar.p Ax₁;
+  q := HasWstar.q Ax₁;
+  r := HasWstar.r Ax₁;
+  mem_Wstar := h mem_Wstar
 
 
 class HasKW1Zero where
@@ -299,22 +299,22 @@ def HasR.of_mem {Ax₁ Ax₂ : Axiom α} (h : Ax₁ ⊆ Ax₂) [Ax₁.HasR] : Ax
   mem_R := h mem_R
 
 
-class HasRStar where
+class HasRstar where
   p : α
   q : α
   r : α
   ne_pq : p ≠ q := by simp;
   ne_qr : q ≠ r := by simp;
   ne_rp : r ≠ p := by simp;
-  mem_RStar : InterpretabilityLogic.Axioms.RStar (.atom p) (.atom q) (.atom r) ∈ Ax := by grind;
-attribute [simp] HasRStar.ne_pq HasRStar.ne_qr HasRStar.ne_rp
-export HasRStar (mem_RStar)
+  mem_Rstar : InterpretabilityLogic.Axioms.Rstar (.atom p) (.atom q) (.atom r) ∈ Ax := by grind;
+attribute [simp] HasRstar.ne_pq HasRstar.ne_qr HasRstar.ne_rp
+export HasRstar (mem_Rstar)
 
-def HasRStar.of_mem {Ax₁ Ax₂ : Axiom α} (h : Ax₁ ⊆ Ax₂) [Ax₁.HasRStar] : Ax₂.HasRStar where
-  p := HasRStar.p Ax₁;
-  q := HasRStar.q Ax₁;
-  r := HasRStar.r Ax₁;
-  mem_RStar := h mem_RStar
+def HasRstar.of_mem {Ax₁ Ax₂ : Axiom α} (h : Ax₁ ⊆ Ax₂) [Ax₁.HasRstar] : Ax₂.HasRstar where
+  p := HasRstar.p Ax₁;
+  q := HasRstar.q Ax₁;
+  r := HasRstar.r Ax₁;
+  mem_Rstar := h mem_Rstar
 
 
 class HasCLAxioms where
