Foundation/InterpretabilityLogic/Veltman/Logic/IL_M.lean
@@ -1,6 +1,5 @@
-import Foundation.InterpretabilityLogic.Veltman.Logic.IL
-import Foundation.InterpretabilityLogic.Veltman.AxiomP
-import Foundation.InterpretabilityLogic.Veltman.Logic.ILRW
+import Foundation.InterpretabilityLogic.Veltman.Logic.IL_R_W
+import Foundation.InterpretabilityLogic.Veltman.AxiomM
 
 namespace LO.InterpretabilityLogic
 
@@ -9,35 +8,35 @@ open Veltman
 
 namespace Veltman
 
-protected class Frame.IsILP (F : Veltman.Frame) extends F.IsIL, F.HasAxiomP
-protected abbrev FrameClass.ILP : FrameClass := { F | F.IsILP }
+protected class Frame.IsILM (F : Veltman.Frame) extends F.IsIL, F.HasAxiomM
+protected abbrev FrameClass.IL_M : FrameClass := { F | F.IsILM }
 
-instance : trivialFrame.IsILP where
-  S_P := by tauto
+instance : trivialFrame.IsILM where
+  S_M := by tauto
 
 end Veltman
 
 
 open Hilbert.Basic
 
-namespace ILP
+namespace ILM
 
-instance Veltman.sound : Sound InterpretabilityLogic.ILP FrameClass.ILP := by
+instance Veltman.sound : Sound InterpretabilityLogic.IL_M FrameClass.IL_M := by
   apply Veltman.instFrameClassSound;
   constructor;
   intro φ hφ F hF;
   replace hF := Set.mem_setOf_eq.mp hF;
   rcases hφ with (rfl | rfl | rfl | rfl | rfl | rfl) <;> simp;
 
-instance : Entailment.Consistent InterpretabilityLogic.ILP := Veltman.consistent_of_sound_frameclass FrameClass.ILP $ by
+instance : Entailment.Consistent InterpretabilityLogic.IL_M := Veltman.consistent_of_sound_frameclass FrameClass.IL_M $ by
   use Veltman.trivialFrame;
   apply Set.mem_setOf_eq.mpr;
   infer_instance;
 
-end ILP
+end ILM
 
 open Entailment in
-instance : InterpretabilityLogic.ILRW ⪱ InterpretabilityLogic.ILP := by
+instance : InterpretabilityLogic.IL_R_W ⪱ InterpretabilityLogic.IL_M := by
   constructor;
   . apply weakerThan_of_provable_axioms;
     intro φ hφ;
@@ -45,21 +44,23 @@ instance : InterpretabilityLogic.ILRW ⪱ InterpretabilityLogic.ILP := by
       axiomJ1, axiomJ2, axiomJ3, axiomJ4, axiomJ5, axiomR, axiomW,
     ];
   . apply Entailment.not_weakerThan_iff.mpr;
-    use (Axioms.P (.atom 0) (.atom 1));
+    use (Axioms.M (.atom 0) (.atom 1) (.atom 2));
     constructor;
     . simp;
-    . apply Sound.not_provable_of_countermodel (𝓜 := Veltman.FrameClass.ILRW);
+    . apply Sound.not_provable_of_countermodel (𝓜 := Veltman.FrameClass.IL_R_W);
       apply Veltman.not_validOnFrameClass_of_exists_frame;
       use {
         toKripkeFrame := {
           World := Fin 4
-          Rel x y := (x = 0 ∧ 0 < y) ∨ (x = 1 ∧ y = 2)
+          Rel x y := (x = 0 ∧ 0 < y) ∨ (x = 2 ∧ y = 3)
         }
         isGL := Modal.Kripke.Frame.isGL_of_isFiniteGL {
           trans := by omega;
           irrefl := by omega;
         }
-        S w x y := (w = 0 ∧ 1 ≤ x ∧ x ≤ y) ∨ (w = 1 ∧ x = 2 ∧ y = 2)
+        S w x y :=
+           (w = 0 ∧ 1 ≤ x ∧ x ≤ y) ∨
+           (w = 2 ∧ x = 3 ∧ y = 3)
         S_cond := by grind;
       }
       constructor;
@@ -69,6 +70,7 @@ instance : InterpretabilityLogic.ILRW ⪱ InterpretabilityLogic.ILP := by
           S_J2 := by grind;
           S_J4 := by grind;
           S_J5 := by grind;
+          S_R := by grind;
           S_W {w} := by
             apply Finite.converseWellFounded_of_trans_irrefl';
             . infer_instance
@@ -78,10 +80,9 @@ instance : InterpretabilityLogic.ILRW ⪱ InterpretabilityLogic.ILP := by
             . dsimp [Irreflexive, Frame.RS, Relation.Comp];
               push_neg;
               grind;
-          S_R := by grind;
         }
       . by_contra hC;
-        have := Veltman.Frame.HasAxiomP.of_validate_axiomP hC |>.S_P (w := 0) (x := 1) (y := 2) (z := 3) (by tauto) (by tauto);
+        have := Veltman.Frame.HasAxiomM.of_validate_axiomM hC |>.S_M (w := 0) (x := 1) (y := 2) (z := 3) (by tauto) (by tauto);
         contradiction;
 
 end LO.InterpretabilityLogic
