Foundation/InterpretabilityLogic/Veltman/Logic/IL_W.lean
@@ -1,0 +1,36 @@
+import Foundation.InterpretabilityLogic.Veltman.Logic.IL_F
+
+namespace LO.InterpretabilityLogic
+
+open Veltman
+
+
+namespace Veltman
+
+protected class Frame.IsIL_W (F : Veltman.Frame) extends F.IsIL, F.HasAxiomW
+protected abbrev FrameClass.IL_W : FrameClass := { F | F.IsIL_W }
+
+instance : trivialFrame.IsIL_W where
+
+end Veltman
+
+
+open Hilbert.Basic
+
+namespace IL_W
+
+instance Veltman.sound : Sound InterpretabilityLogic.IL_W FrameClass.IL_W := by
+  apply Veltman.instFrameClassSound;
+  constructor;
+  intro φ hφ F hF;
+  replace hF := Set.mem_setOf_eq.mp hF;
+  rcases hφ with (rfl | rfl | rfl | rfl | rfl | rfl) <;> simp;
+
+instance : Entailment.Consistent InterpretabilityLogic.IL_W := Veltman.consistent_of_sound_frameclass FrameClass.IL_W $ by
+  use Veltman.trivialFrame;
+  apply Set.mem_setOf_eq.mpr;
+  infer_instance;
+
+end IL_W
+
+end LO.InterpretabilityLogic
