Zoo/InterpretabilityLogic.typ
@@ -21,21 +21,33 @@
   }
 })
 
-#let ILMinus = $Logic("IL"^-)$
+#let LogicILMinus = $Logic("IL"^-)$
+#let LogicIL = $Logic("IL")$
+#let LogicCL = $Logic("CL")$
 #let AxiomJ1 = $Axiom("J1")$
 #let AxiomJ2 = $Axiom("J2")$
 #let AxiomJ2Plus = $Axiom("J2"^+)$
 #let AxiomJ4 = $Axiom("J4")$
 #let AxiomJ4Plus = $Axiom("J4"^+)$
 #let AxiomJ5 = $Axiom("J5")$
-
+#let AxiomF = $Axiom("F")$
+#let AxiomM = $Axiom("M")$
+#let AxiomM0 = $Axiom("M"_0)$
+#let AxiomW = $Axiom("W")$
+#let AxiomP = $Axiom("P")$
+#let AxiomP0 = $Axiom("P"_0)$
+#let AxiomR = $Axiom("R")$
+#let AxiomKW1Zero = $Axiom("KW1"^0)$
+#let AxiomKW2 = $Axiom("KW2")$
+#let AxiomRstar = $Axiom("R"^*)$
+#let AxiomWstar = $Axiom("W"^*)$
 
 #figure(caption: [Interpretability Logic Zoo], numbering: none)[
   #raw-render(
     raw(
       "
   digraph ModalTheorysZoo {
-    rankdir = RL;
+    rankdir = TB;
 
     node [
       shape=none
@@ -54,35 +66,35 @@
         + "}",
     ),
     labels: (
-      "LO.InterpretabilityLogic.CL": $Logic("CL")$,
-      "LO.InterpretabilityLogic.IL_KW1Zero": $Logic("IL")(Axiom("KW1"^0))$,
-      "LO.InterpretabilityLogic.IL_KW2": $Logic("IL")(Axiom("KW2"))$,
-      "LO.InterpretabilityLogic.IL": $Logic("IL")$,
-      "LO.InterpretabilityLogic.ILF": $Logic("ILF")$,
-      "LO.InterpretabilityLogic.ILM": $Logic("ILM")$,
-      "LO.InterpretabilityLogic.ILM₀": $Logic("IL"M_0)$,
-      "LO.InterpretabilityLogic.ILP": $Logic("ILP")$,
-      "LO.InterpretabilityLogic.ILP₀": $Logic("ILP"_0)$,
-      "LO.InterpretabilityLogic.ILR": $Logic("ILR")$,
-      "LO.InterpretabilityLogic.ILRStar": $Logic("IL"R^*)$,
-      "LO.InterpretabilityLogic.ILRW": $Logic("ILRW")$,
-      "LO.InterpretabilityLogic.ILW": $Logic("ILW")$,
-      "LO.InterpretabilityLogic.ILWM₀": $Logic("ILW"M_0)$,
-      "LO.InterpretabilityLogic.ILWStar": $Logic("IL"W^*)$,
-      "LO.InterpretabilityLogic.ILMinus_J1_J2_J5": $ILMinus (AxiomJ1, AxiomJ2, AxiomJ5)$,
-      "LO.InterpretabilityLogic.ILMinus_J1_J2": $ILMinus (AxiomJ1, AxiomJ2)$,
-      "LO.InterpretabilityLogic.ILMinus_J1_J4Plus_J5": $ILMinus (AxiomJ1, AxiomJ4Plus, AxiomJ5)$,
-      "LO.InterpretabilityLogic.ILMinus_J1_J4Plus": $ILMinus (AxiomJ1, AxiomJ4Plus)$,
-      "LO.InterpretabilityLogic.ILMinus_J1_J5": $ILMinus (AxiomJ1, AxiomJ5)$,
-      "LO.InterpretabilityLogic.ILMinus_J1": $ILMinus (AxiomJ1)$,
-      "LO.InterpretabilityLogic.ILMinus_J2Plus_J5": $ILMinus (AxiomJ2Plus, AxiomJ5)$,
-      "LO.InterpretabilityLogic.ILMinus_J2Plus": $ILMinus (AxiomJ2Plus)$,
-      "LO.InterpretabilityLogic.ILMinus_J4": $ILMinus (AxiomJ4)$,
-      "LO.InterpretabilityLogic.ILMinus_J4Plus_J5": $ILMinus (AxiomJ4Plus, AxiomJ5)$,
-      "LO.InterpretabilityLogic.ILMinus_J4Plus": $ILMinus (AxiomJ4Plus)$,
-      "LO.InterpretabilityLogic.ILMinus_J5": $ILMinus (AxiomJ5)$,
-      "LO.InterpretabilityLogic.ILMinus": $ILMinus$,
+      "LO.InterpretabilityLogic.CL": $LogicCL$,
+      "LO.InterpretabilityLogic.IL_F": $LogicIL(AxiomF)$,
+      "LO.InterpretabilityLogic.IL_KW1Zero": $LogicIL(AxiomKW1Zero)$,
+      "LO.InterpretabilityLogic.IL_KW2": $LogicIL(AxiomKW2)$,
+      "LO.InterpretabilityLogic.IL_M": $LogicIL(AxiomM)$,
+      "LO.InterpretabilityLogic.IL_M₀_W": $LogicIL(AxiomM0, AxiomW)$,
+      "LO.InterpretabilityLogic.IL_M₀": $LogicIL(AxiomM0)$,
+      "LO.InterpretabilityLogic.IL_P": $LogicIL(AxiomP)$,
+      "LO.InterpretabilityLogic.IL_P₀": $LogicIL(AxiomP0)$,
+      "LO.InterpretabilityLogic.IL_R_W": $LogicIL(AxiomR, AxiomW)$,
+      "LO.InterpretabilityLogic.IL_R": $LogicIL(AxiomR)$,
+      "LO.InterpretabilityLogic.IL_Rstar": $LogicIL(AxiomRstar)$,
+      "LO.InterpretabilityLogic.IL_W": $LogicIL(AxiomW)$,
+      "LO.InterpretabilityLogic.IL_Wstar": $LogicIL(AxiomWstar)$,
+      "LO.InterpretabilityLogic.IL": $LogicIL$,
+      "LO.InterpretabilityLogic.ILMinus_J1_J2_J5": $LogicILMinus(AxiomJ1, AxiomJ2, AxiomJ5)$,
+      "LO.InterpretabilityLogic.ILMinus_J1_J2": $LogicILMinus(AxiomJ1, AxiomJ2)$,
+      "LO.InterpretabilityLogic.ILMinus_J1_J4Plus_J5": $LogicILMinus(AxiomJ1, AxiomJ4Plus, AxiomJ5)$,
+      "LO.InterpretabilityLogic.ILMinus_J1_J4Plus": $LogicILMinus(AxiomJ1, AxiomJ4Plus)$,
+      "LO.InterpretabilityLogic.ILMinus_J1_J5": $LogicILMinus(AxiomJ1, AxiomJ5)$,
+      "LO.InterpretabilityLogic.ILMinus_J1": $LogicILMinus(AxiomJ1)$,
+      "LO.InterpretabilityLogic.ILMinus_J2Plus_J5": $LogicILMinus(AxiomJ2Plus, AxiomJ5)$,
+      "LO.InterpretabilityLogic.ILMinus_J2Plus": $LogicILMinus(AxiomJ2Plus)$,
+      "LO.InterpretabilityLogic.ILMinus_J4": $LogicILMinus(AxiomJ4)$,
+      "LO.InterpretabilityLogic.ILMinus_J4Plus_J5": $LogicILMinus(AxiomJ4Plus, AxiomJ5)$,
+      "LO.InterpretabilityLogic.ILMinus_J4Plus": $LogicILMinus(AxiomJ4Plus)$,
+      "LO.InterpretabilityLogic.ILMinus_J5": $LogicILMinus(AxiomJ5)$,
+      "LO.InterpretabilityLogic.ILMinus": $LogicILMinus$,
     ),
-    width: 640pt,
+    width: 320pt,
   )
 ]
